dh.v
@@ -81,69 +81,33 @@ rewrite public_TExp1; do !iSplit => //.
 by iRight; iApply "aP"; iModIntro; iExists _, _; eauto.
 Qed.
 
-Definition dh_meta `{Countable L} t N (x : L) : iProp :=
-  (∃ g a, ⌜t = TExp g [a]⌝ ∧ nonce_meta a N x)%I.
-
-Definition dh_meta_token t E : iProp :=
-  (∃ g a, ⌜t = TExp g [a]⌝ ∧ nonce_meta_token a E)%I.
-
-Program Global Instance dh_term_meta :
-  TermMeta (@dh_meta) dh_meta_token.
-
-Next Obligation.
-iIntros (L ?? E t x N sub).
-iDestruct 1 as (g a) "[-> token]".
-iMod (term_meta_set _ _ x with "token") as "meta"; eauto.
-by rewrite /dh_meta; eauto.
-Qed.
-
-Next Obligation.
-iIntros (L ?? t x N E sub).
-iDestruct 1 as (g a) "[-> token]".
-iDestruct 1 as (??)  "[%e  meta]".
-case/TExp_inj1: e => _ <-.
-by iApply (term_meta_meta_token with "token meta").
-Qed.
-
-Next Obligation.
-iIntros (L ?? t N x1 x2).
-iDestruct 1 as (g a) "[-> meta1]".
-iDestruct 1 as (??)  "[%e meta2]".
-case/TExp_inj1: e => _ <-.
-by iApply (term_meta_agree with "meta1 meta2").
-Qed.
-
-Next Obligation.
-rewrite /dh_meta /dh_meta_token.
-move=> t E1 E2 sub; iSplit.
-- iDestruct 1 as (g a) "[-> token]".
-  rewrite [nonce_meta_token _ _](term_meta_token_difference a E1 E2) //.
-  by iDestruct "token" as "[token1 token2]"; iSplitL "token1"; eauto.
-- iDestruct 1 as "[token1 token2]".
-  iDestruct "token1" as (g a) "[-> token1]".
-  iDestruct "token2" as (??) "[%e token2]".
-  case/TExp_inj1: e => _ <-.
-  iExists _, _; iSplit => //.
-  rewrite (term_meta_token_difference _ E1 E2) //.
-  by iSplitL "token1".
-Qed.
-
 Definition mkdh : val := mknonce.
 
 Lemma wp_mkdh g E (Ψ : val → iProp) :
+  ↑cryptisN ⊆ E →
+  cryptis_ctx -∗
+  minted g -∗
   (∀ a, minted a -∗
         dh_seed a -∗
-        dh_meta_token (TExp g [a]) ⊤ -∗
+        term_token (TExp g [a]) ⊤ -∗
         Ψ a) -∗
   WP mkdh #() @ E {{ Ψ }}.
 Proof.
-iIntros "post"; iApply (wp_mknonce (λ _, False%I) dh_publ).
-iIntros (a) "#s_a #(aP1 & aP2) #? token"; iApply "post" => //.
-do !iSplit => //.
+iIntros "% #ctx #minted_g post".
+iApply (wp_mknonce_freshN ∅ (λ _, False%I) dh_publ (λ t, {[TExp g [t]]})
+  with "[//]" ) => //.
+- iIntros "%". rewrite elem_of_empty. by iIntros "[]".
+- iIntros "%". rewrite big_sepS_singleton. iIntros "!>".
+  rewrite minted_TExp /=.
+  iSplit.
+  + by iIntros "?"; do !iSplit.
+  + by iIntros "(? & ? & ?)".
+iIntros (a) "_ #m_a #(aP1 & aP2) #? token". rewrite big_sepS_singleton.
+iApply "post" => //.
+rewrite /dh_seed. do !iSplit => //.
 iModIntro; iSplit.
 - by iIntros "H"; iSpecialize ("aP1" with "H"); iModIntro.
 - by iIntros "#?"; iApply "aP2"; iModIntro.
-- by iExists g, a; eauto.
 Qed.
 
 End DH.
